Signature_Examples.thy
@@ -217,7 +217,7 @@ qed
 
 end
 
-text \<open>We must define the following four constants outside the global interpretation, since otherwise
+text \<open>We must define the following two constants outside the global interpretation, since otherwise
   their types are too general.\<close>
 
 definition splus_pprod :: "('a::nat, 'b::nat) pp \<Rightarrow> _"
@@ -258,6 +258,7 @@ global_interpretation pprod': qpm_nat_inf_term to
   and new_syz_sigs_spp_pprod = pprod'.aux.new_syz_sigs_spp
   and sig_gb_spp_body_pprod = pprod'.aux.sig_gb_spp_body
   and sig_gb_spp_aux_pprod = pprod'.aux.sig_gb_spp_aux
+  and sig_gb_z_pprod' = pprod'.aux.sig_gb_z
   and sig_gb_pprod' = pprod'.aux.sig_gb
   and rw_rat_strict_pprod = pprod'.aux.rw_rat_strict
   and rw_add_strict_pprod = pprod'.aux.rw_add_strict
@@ -296,7 +297,7 @@ lemma compute_sig_trd_spp_pprod [code]:
 
 lemmas [code] = conversep_iff
 
-lemma is_pot_ord [code]:
+lemma compute_is_pot_ord [code]:
   "is_pot_ord_pprod (LEX::(('a::nat, 'b::nat) pp \<times> nat) nat_term_order) = False"
     (is "is_pot_ord_pprod ?lex = _")
   "is_pot_ord_pprod (DRLEX::(('a::nat, 'b::nat) pp \<times> nat) nat_term_order) = False"
@@ -355,22 +356,37 @@ proof -
   thus "is_pot_ord_pprod (POT to) = True" by simp
 qed
 
+corollary is_pot_ord_POT: "is_pot_ord_pprod (POT to)"
+  by (simp only: compute_is_pot_ord)
+
+definition "sig_gb_z_pprod to rword_strict fs \<equiv>
+                  (let res = sig_gb_z_pprod' to (rword_strict to) (map (change_ord (proj_ord to)) fs) in
+                    (length (fst res), snd res))"
+
 definition "sig_gb_pprod to rword_strict fs \<equiv> sig_gb_pprod' to (rword_strict to) (map (change_ord (proj_ord to)) fs)"
+
+lemma snd_sig_gb_z_pprod'_eq_sig_gb_z_pprod:
+  "snd (sig_gb_z_pprod' to (rword_strict to) fs) = snd (sig_gb_z_pprod to rword_strict fs)"
+  by (simp add: sig_gb_z_pprod_def change_ord_def Let_def)
 
 lemma sig_gb_pprod'_eq_sig_gb_pprod:
   "sig_gb_pprod' to (rword_strict to) fs = sig_gb_pprod to rword_strict fs"
   by (simp add: sig_gb_pprod_def change_ord_def)
 
-thm pprod'.aux.sig_gb[OF pprod'.aux.rw_rat_strict_is_strict_rewrite_ord, simplified sig_gb_pprod'_eq_sig_gb_pprod]
+thm pprod'.aux.sig_gb_isGB[OF pprod'.aux.rw_rat_strict_is_strict_rewrite_ord, simplified sig_gb_pprod'_eq_sig_gb_pprod]
+thm pprod'.aux.sig_gb_no_zero_red[OF pprod'.aux.rw_rat_strict_is_strict_rewrite_ord is_pot_ord_POT, simplified snd_sig_gb_z_pprod'_eq_sig_gb_z_pprod]
 
-lemma sig_gb_spp_body_pprod_code [code]:
-  "sig_gb_spp_body_pprod to fs rword_strict (bs, ss, p # ps) =
+(*
+lemma sig_gb_spp_body_pprod_code_print [code]:
+  "sig_gb_spp_body_pprod to fs rword_strict ((bs, ss, p # ps), z) =
   (let ss' = new_syz_sigs_spp_pprod to fs ss bs p
-  in if sig_crit_spp_pprod to rword_strict bs ss' p then (bs, ss', ps)
+  in if sig_crit_spp_pprod to rword_strict bs ss' p then ((bs, ss', ps), z)
      else let p' = sig_trd_spp_pprod to bs (spp_of_pair_pprod to fs p)
-          in if snd p' = 0 then print ''0'' (bs, fst p' # ss', ps) else (p' # bs, ss', add_spairs_spp_pprod to ps bs p'))"
-  "sig_gb_spp_body_pprod to fs rword_strict (bs, ss, []) = (bs, ss, [])"
+          in if snd p' = 0 then print ''0'' ((bs, fst p' # ss', ps), Suc z)
+              else ((p' # bs, ss', add_spairs_spp_pprod to ps bs p'), z))"
+  "sig_gb_spp_body_pprod to fs rword_strict ((bs, ss, []), z) = ((bs, ss, []), z)"
   by (simp_all add: Let_def)
+*)
 
 subsection \<open>Computations\<close>
 
@@ -394,14 +410,14 @@ value [code] "rw_rat_strict_pprod DRLEX ((0, 0), poly1) ((0, 0), poly2)"
 
 value [code] "rw_add_strict_pprod DRLEX ((0, 0), poly1) ((0, 0), poly2)"
 
-value [code] "sig_gb_spp_body_pprod DRLEX ((cyclic DRLEX 2)::(_ \<Rightarrow>\<^sub>0 rat) list) (rw_rat_strict_pprod DRLEX) ([], [], [Inr 0, Inr 1])"
+value [code] "sig_gb_spp_body_pprod DRLEX ((cyclic DRLEX 2)::(_ \<Rightarrow>\<^sub>0 rat) list) (rw_rat_strict_pprod DRLEX) (([], [], [Inr 0, Inr 1]), 0)"
 
 text \<open>We restrict computations of (signature) Gr\"obner bases to @{const rw_rat_strict_pprod}, because
   according to @{thm pprod'.aux.sig_gb_aux_is_min_sig_GB} this rewrite-order is optimal.\<close>
 
 value [code] "sig_gb_pprod DRLEX rw_rat_strict_pprod [poly1, poly2]"
 
-value [code] "timing (length (sig_gb_pprod (POT DRLEX) rw_rat_strict_pprod ((Katsura DRLEX 1)::(_ \<Rightarrow>\<^sub>0 rat) list)))"
+value [code] "timing ((sig_gb_z_pprod (POT DRLEX) rw_rat_strict_pprod ((cyclic DRLEX 1)::(_ \<Rightarrow>\<^sub>0 rat) list)))"
 
 (*
 Timings on benchmark problems
@@ -431,6 +447,10 @@ Cyclic-7      996.6            ?         177            (on qftquad4)
 Katsura-4       0.0           16          11
 Katsura-5       1.0           32          26
 Katsura-6      28.1           64          57
+
+First experiments with the finite field of order 32003 indicate that "rat" is faster, probably
+because of the non-optimal implementation of division in the finite field and of "mod" in the
+underlying ring of integers.
 *)
 
 (* https://raw.githubusercontent.com/ederc/singular-benchmarks/master/benchs.lib *)
